src/program_proof/txn/specs.v
@@ -39,9 +39,9 @@ Definition mapsto_txn {K} (gData : gmap u64 (sigT (fun K => gen_heapG u64 (updat
     mapsto (hG := hG) a.(addrOff) 1 (UB v γm) ∗
     own γm (◯ (Excl' true)).
 
-Theorem mapsto_txn_2 {K} gData a v0 v1 :
-  @mapsto_txn K gData a v0 -∗
-  @mapsto_txn K gData a v1 -∗
+Theorem mapsto_txn_2 {K1 K2} gData a v0 v1 :
+  @mapsto_txn K1 gData a v0 -∗
+  @mapsto_txn K2 gData a v1 -∗
   False.
 Proof.
   rewrite /mapsto_txn.
@@ -49,8 +49,9 @@ Proof.
   iDestruct "H0" as (g0 m0) "(% & % & H0m & H0own)".
   iDestruct "H1" as (g1 m1) "(% & % & H1m & H1own)".
   rewrite H0 in H2; inversion H2.
-  apply eq_sigT_eq_dep in H4.
-  apply Eqdep_dec.eq_dep_eq_dec in H4; subst.
+  subst.
+  apply eq_sigT_eq_dep in H5.
+  apply Eqdep_dec.eq_dep_eq_dec in H5; subst.
   2: apply bufDataKind_eq_dec.
   iDestruct (mapsto_valid_2 with "H0m H1m") as %x.
   exfalso; eauto.
